Cleanup

theories/L6_PCPS/closure_conversion_correct.v
@@ -2,10 +2,9 @@
  * Author: Zoe Paraskevopoulou, 2016
  *)
 
-Require Import L6.tactics.
+Require Import L6.tactics L6.closure_conversion_invariants L6.closure_conversion L6.closure_conversion_util.
 From CertiCoq.L6 Require Import cps size_cps cps_util set_util hoisting identifiers ctx
-                       Ensembles_util List_util functions closure_conversion
-                       closure_conversion_util eval logical_relations.
+                       Ensembles_util List_util functions eval logical_relations_cc.
 Require Import compcert.lib.Coqlib.
 From Coq Require Import ZArith.Znumtheory Relations.Relations Arith.Wf_nat
                         Lists.List MSets.MSets MSets.MSetRBT Numbers.BinNums
@@ -17,34 +16,6 @@ Open Scope ctx_scope.
 Open Scope fun_scope.
 Close Scope Z_scope.
 
-(** For closure conversion, the free variables of an expression are divided in
-    three categories :
-
-    1. Variables in the current scope, i.e. arguments of the current function
-    and bindings in the body of the current function definition.
-
-    2. Names of the functions that are defined in the current block of mutually
-    recursive functions.
-
-    3. Free variables, i.e. variables that are not declared outside of the
-    body of the current function but in outer definitions
-
-    In the proof maintains different invariants for each kind of variable *)
-
-
-(** * Invariants *)
-
-(** Naming conventions in the following :
-
-    [Scope] : The set of variables in the current scope.
-
-    [Funs] : The set of variables in the current block of mutually recursive
-    functions.
-
-    [FVs] : The list of free variables (needs to be ordered).
-
-    [Γ] : The formal parameter of the environment after closure conversion. *)
-
 
 Section Closure_conversion_correct.
 
@@ -52,783 +23,21 @@ Section Closure_conversion_correct.
   Variable cenv : ctor_env.
   Variable clo_tag : ctor_tag.
 
-
+  (* Parameterize over the postconditions *)
+  Context (boundL : nat -> exp -> env -> relation nat)
+          (boundG : nat -> relation (exp * env * nat)).
+  
   (** ** Semantics preservation proof *)
 
   (** We show observational approximation of the final results as well as an
     * upper bound on the concrete execution cost of the translated program *)
-
-
-  (** *  Useful definitions and lemmas to express the upper bound. *)
-
-  Definition max_exp_env (k : nat) (e : exp) (rho : env) :=
-    max (sizeOf_exp e) (sizeOf_env k rho).
-
   
-  Lemma max_exp_env_grt_1 k e rho :
-    1 <= max_exp_env k e rho.
-  Proof.
-    unfold max_exp_env.
-    eapply le_trans. now apply sizeOf_exp_grt_1.
-    eapply Max.le_max_l.
-  Qed.
-
-  (** Lemmas used to establish the upper bound given the IH *)
-
-  Lemma max_exp_env_Econstr k x t ys e rho :
-    max_exp_env k e rho <= max_exp_env k (Econstr x t ys e) rho.
-  Proof.
-    eapply NPeano.Nat.max_le_compat_r.
-    simpl. omega.
-  Qed.
-
-  Lemma max_exp_env_Eproj k x t N y e rho :
-    max_exp_env k e rho <= max_exp_env k (Eproj x t N y e) rho.
-  Proof.
-    eapply NPeano.Nat.max_le_compat_r.
-    simpl. omega.
-  Qed.
-
-  Lemma max_exp_env_Ecase_cons_hd k x c e l rho :
-    max_exp_env k e rho <= max_exp_env k (Ecase x ((c, e) :: l)) rho.
-  Proof.
-    eapply NPeano.Nat.max_le_compat_r.
-    simpl. omega.
-  Qed.
-
-  Lemma max_exp_env_Ecase_cons_tl k x c e l rho :
-    max_exp_env k (Ecase x l) rho <= max_exp_env k (Ecase x ((c, e) :: l)) rho.
-  Proof.
-    eapply NPeano.Nat.max_le_compat_r.
-    simpl. omega.
-  Qed.
-
-  Lemma max_exp_env_Eprim k x f ys e rho :
-    max_exp_env k e rho <= max_exp_env k (Eprim x f ys e) rho.
-  Proof.
-    eapply NPeano.Nat.max_le_compat_r.
-    simpl. omega.
-  Qed.
-
-  Lemma max_exp_env_Efun k B e rho :
-    max_exp_env k e (def_funs B B rho rho) <= max_exp_env k (Efun B e) rho.
-  Proof.
-    unfold max_exp_env. eapply le_trans.
-    - eapply NPeano.Nat.max_le_compat_l.
-      now apply sizeOf_env_def_funs.
-    - rewrite (Max.max_comm (sizeOf_env _ _)), Max.max_assoc.
-      eapply NPeano.Nat.max_le_compat_r.
-      eapply Nat.max_lub; simpl; omega.
-  Qed.
-
-  (** * Definition of the bounds *)
-
-  (** Local predicate. Enforced only for the cost of the particular expressions
-    * related. It's likely that the upper bound can be refined further *)
-
-  Definition upper_boundL := 
-    fun i (e1 : exp) (rho1 : env) (c1 c2 : nat) =>
-      c2 <= 8 * c1 * (max_exp_env i e1 rho1) + 8 * sizeOf_exp e1.
-
-  Definition lower_boundL := 
-    fun (c1 c2 : nat) => c1 <= c2.
+  (* Short-hands so that we don't have to apply the parameters every time *)
+  Definition FV_inv := FV_inv pr cenv clo_tag boundG. 
+  Definition Fun_inv := Fun_inv pr cenv clo_tag boundG. 
+  Definition GFun_inv := GFun_inv pr cenv clo_tag boundG. 
+  Definition closure_env := closure_env pr cenv clo_tag boundG. 
   
-  Definition boundL (i : nat) (e1 : exp) (rho1 : env) (c1 : nat) (c2 : nat) : Prop :=
-    lower_boundL c1 c2 /\ upper_boundL i e1 rho1 c1 c2.
-  
-  (* Global predicate. Enforced on values.  *)
-  Definition boundG (k : nat) (p1 : exp * env * nat) (p2 : exp * env * nat) : Prop :=
-    let '(e1, rho1, c1) := p1 in
-    let '(e2, rho2, c2) := p2 in
-    boundL k e1 rho1 c1 c2.
-  
-  (** Invariant about the values of free variables. *)
-  Definition closure_env k rho Scope Funs GFuns vs FVs : Prop :=
-      Forall2 (fun x v' => 
-                 forall v, ~ In _ Scope x ->
-                      ~ In _ Funs x ->
-                      ~ In _ GFuns x ->
-                      M.get x rho = Some v ->
-                      cc_approx_val pr cenv clo_tag k boundG v v') FVs vs.
-  
-  (** Invariant about the free variables *) 
-  Definition FV_inv k rho rho' Scope Funs GFuns c Γ FVs : Prop :=
-    exists c' (vs : list val),
-      M.get Γ rho' = Some (Vconstr c' vs) /\
-      (FVs <> [] -> c' = c) /\ (* Because if FVs = [] we don't care about c' *)
-      Forall2 (fun x v' => 
-                 forall v, ~ In _ Scope x ->
-                      ~ In _ Funs x ->
-                      ~ In _ GFuns x ->
-                      M.get x rho = Some v ->
-                      cc_approx_val pr cenv clo_tag k boundG v v') FVs vs.
-  
-  (** Invariant about the functions in the current function definition *)
-  Definition Fun_inv k (rho rho' : env) Scope Funs σ Γ : Prop :=
-    forall f v,
-      ~ In _ Scope f ->
-      In var Funs f ->
-      M.get f rho = Some v  ->
-      exists env rho1 B1 f1 rho2 B2 f2,
-        M.get Γ rho' = Some env /\
-        v = (Vfun rho1 B1 f1) /\
-        ~ In _ Scope (σ f) /\
-        M.get (σ f) rho' = Some (Vfun rho2 B2 f2) /\
-        cc_approx_val pr cenv clo_tag k boundG
-                      (Vfun rho1 B1 f1)
-                      (Vconstr clo_tag [(Vfun rho2 B2 f2) ; env]).
-
-  (** Invariant about the functions in the current function definition *)
-  Definition GFun_inv k (rho rho' : env) Scope GFuns σ : Prop :=
-    forall f v c,
-      In var GFuns f ->
-      M.get f rho = Some v  ->
-      exists rho1 B1 f1 rho2 B2 f2,
-        v = (Vfun rho1 B1 f1) /\
-        ~ In _ Scope (σ f) /\ (* Check if needed *)
-        M.get (σ f) rho' = Some (Vfun rho2 B2 f2) /\
-        cc_approx_val pr cenv clo_tag k boundG
-                      (Vfun rho1 B1 f1)
-                      (Vconstr clo_tag [(Vfun rho2 B2 f2) ; (Vconstr c [])]).
-
-
-  (** * Lemmas about Fun_inv *)
-
-  (** Extend the two environments with a variable that is not the current environment
-    argument (i.e. [Γ]) *)
-  Lemma Fun_inv_set k rho rho' Scope Funs σ Γ f rho1 B1 f1 rho2 B2 f2 env:
-    Fun_inv k rho rho' Scope Funs σ Γ ->
-    (σ f) <> Γ ->
-    ~ In _ Scope (σ f) ->
-    ~ In _ (image σ (Setminus _ Funs Scope)) (σ f) ->
-    M.get Γ rho' = Some env ->
-    (cc_approx_val pr cenv clo_tag k boundG (Vfun rho1 B1 f1)
-                   (Vconstr clo_tag [(Vfun rho2 B2 f2) ; env])) ->
-    Fun_inv k (M.set f (Vfun rho1 B1 f1) rho)
-            (M.set (σ f) (Vfun rho2 B2 f2) rho')
-            Scope (Union _ (Singleton _ f) Funs) σ Γ.
-  Proof.
-    intros Hinv Hneq Hnin Hnin' Hget Hv f'' v Hnin'' Hin Hget'.
-    destruct (peq f'' f); subst.
-    - repeat eexists; eauto. rewrite M.gso; eauto.
-      now rewrite M.gss in Hget'; inv Hget'; eauto.
-      now rewrite M.gss.
-    - inv Hin. inv H; congruence. rewrite M.gso in Hget'; eauto.
-      edestruct Hinv with (f := f'') as
-          [vs' [rho3 [B3 [f3 [rho4 [B4 [f4 [Hget1 [Heq2 [Ηnin2 [Hget2 Happrox]]]]]]]]]]];
-        subst; eauto.
-      repeat eexists; eauto. rewrite M.gso; now eauto. 
-      rewrite M.gso. now eauto.
-      intros Hc. eapply Hnin'. eexists; eauto. split; [| eassumption ].
-      now constructor; eauto.
-  Qed.
-
-  (** Rename the environment parameter *)
-  Lemma Fun_inv_rename k rho1 rho2 Scope Funs σ Γ Γ' v :
-    ~ In _ (image σ (Setminus _ Funs Scope)) Γ ->  ~ In _ (image σ Funs) Γ' ->
-    Fun_inv k rho1 (M.set Γ v rho2) Scope Funs σ Γ ->
-    Fun_inv k rho1 (M.set Γ' v rho2) Scope Funs σ Γ'.
-  Proof.
-    intros Hnin Hnin' Hinv f v1 Hninf Hinf Hget.
-    edestruct Hinv with (f := f) as
-        [vs' [rho3 [B3 [f3 [rho4 [B4 [f4 [Hget1 [Heq2 [Ηnin2 [Hget2 Happrox]]]]]]]]]]]; eauto.
-    rewrite M.gss in Hget1. inv Hget1.
-    repeat eexists; eauto. now rewrite M.gss; eauto.
-    rewrite M.gso in Hget2. rewrite M.gso; eauto.
-    intros Hc. eapply Hnin'. now eexists; split; eauto.
-    intros Hc. eapply Hnin. now eexists; split; eauto.
-  Qed.
-  
-  (** Extend [Scope] with a set that does not shadow the new function names *)
-  Lemma Fun_inv_mon k rho1 rho2 Scope Scope' Funs σ Γ :
-    Disjoint _ (image σ (Setminus _ Funs Scope)) Scope' ->
-    Fun_inv k rho1 rho2 Scope Funs σ Γ ->
-    Fun_inv k rho1 rho2 (Union _ Scope' Scope) Funs σ Γ.
-  Proof.
-    intros Hd Hinv f v Hninf Hinf Hget.
-    edestruct Hinv with (f := f) as
-        [vs' [rho3 [B3 [f3 [rho4 [B4 [f4 [Hget1 [Heq2 [Ηnin2 [Hget2 Happrox]]]]]]]]]]]; eauto.
-    repeat eexists; eauto.
-    intros Hc; inv Hc. eapply Hd. constructor; eauto. 
-    eexists; eauto. split; [| now eauto ]. now constructor; eauto.
-    now eauto.
-  Qed.
-
-  (** Extend the first environment with a variable in [Scope] *)
-  Lemma Fun_inv_set_In_Scope_l k rho1 rho2 Scope Funs σ Γ x v :
-    In _ Scope x ->
-    Fun_inv k rho1 rho2 Scope Funs σ Γ ->
-    Fun_inv k (M.set x v rho1) rho2 Scope Funs σ Γ.
-  Proof.
-    intros Hin Hinv f v' Hninf Hinf Hget.
-    eapply Hinv; eauto. rewrite M.gso in Hget.
-    now eauto. intros Hc; subst. now eauto.
-  Qed.
-
-    (** Extend the first environment with a variable in not in [Funs] *)
-  Lemma Fun_inv_set_not_In_Funs_l k rho1 rho2 Scope Funs σ Γ x v :
-    ~ In _ Funs x  ->
-    Fun_inv k rho1 rho2 Scope Funs σ Γ ->
-    Fun_inv k (M.set x v rho1) rho2 Scope Funs σ Γ.
-  Proof.
-    intros Hin Hinv f v' Hninf Hinf Hget.
-    eapply Hinv; eauto. rewrite M.gso in Hget.
-    now eauto. intros Hc; subst. now eauto.
-  Qed.
-
-  (** Extend the first environment with a variable in not in [Funs] *)
-  Lemma Fun_inv_funs_monotonic k rho1 rho2 Scope Funs Funs' σ Γ :
-    Fun_inv k rho1 rho2 Scope Funs σ Γ ->
-    Funs' \subset Funs -> 
-    Fun_inv k rho1 rho2 Scope Funs' σ Γ.
-  Proof.
-    intros Hin Hinv f v' Hninf Hinf Hget.
-    eapply Hin; eauto.
-  Qed.
-  
-  (** Extend the second environment with a variable in [Scope] *)
-  Lemma Fun_inv_set_In_Scope_r k rho1 rho2 Scope Funs σ Γ x v v' :
-    In _ Scope x ->  ~ In _ (image σ (Setminus _ Funs Scope)) x ->
-    Fun_inv k rho1 (M.set Γ v rho2) Scope Funs σ Γ ->
-    Fun_inv k rho1 (M.set Γ v (M.set x v' rho2)) Scope Funs σ Γ.
-  Proof.
-    intros Hin Hnin Hinv f v1 Hninf Hinf Hget.
-    edestruct Hinv with (f := f) as
-        [vs' [rho3 [B3 [f3 [rho4 [B4 [f4 [Hget1 [Heq2 [Ηnin2 [Hget2 Happrox]]]]]]]]]]]; eauto.
-    rewrite M.gss in Hget1; inv Hget1. 
-    repeat eexists; eauto. now rewrite M.gss.
-    destruct (peq (σ f) Γ).
-    - subst. now rewrite M.gss in *.
-    - rewrite M.gso; eauto. rewrite M.gso in Hget2; eauto.
-      rewrite M.gso; eauto.
-      intros Hc; subst. eapply Hnin. eexists; eauto.
-      split; [| now eauto]. constructor; eauto.
-  Qed.
-
-  (** Extend the second environment with a variable in [Scope] that is different
-    from [Γ] *)
-  Lemma Fun_inv_set_In_Scope_r_not_Γ k rho1 rho2 Scope Funs σ Γ x v :
-    In _ Scope x -> Γ <> x ->
-    Fun_inv k rho1 rho2 Scope Funs σ Γ ->
-    Fun_inv k rho1 (M.set x v rho2) Scope Funs σ Γ.
-  Proof.
-    intros Hin Hnin Hinv f v1 Hninf Hinf Hget.
-    edestruct Hinv with (f := f) as
-        [vs' [rho3 [B3 [f3 [rho4 [B4 [f4 [Hget1 [Heq2 [Ηnin2 [Hget2 Happrox]]]]]]]]]]]; eauto.
-    repeat eexists; eauto.
-    now rewrite M.gso.
-    rewrite M.gso. now eauto.
-    intros Hc. subst. contradiction.
-  Qed.  
-
-  (** Extend the second environment with a variable not in [Funs] that is different
-    from Γ *)
-  Lemma Fun_inv_set_not_In_Funs_r_not_Γ k rho1 rho2 Scope Funs σ Γ x v :
-    ~ In _ (image σ (Setminus _ Funs Scope)) x ->
-    x <> Γ -> 
-    Fun_inv k rho1 rho2 Scope Funs σ Γ ->
-    Fun_inv k rho1 (M.set x v rho2) Scope Funs σ Γ.
-  Proof.
-    intros Hnin Hneq Hinv f v1 Hninf Hinf Hget.
-    edestruct Hinv with (f := f) as
-        [vs' [rho3 [B3 [f3 [rho4 [B4 [f4 [Hget1 [Heq2 [Ηnin2 [Hget2 Happrox]]]]]]]]]]]; eauto.
-    repeat eexists; eauto.
-    rewrite M.gso. now eauto.
-    intros Hc. subst. congruence.
-    rewrite M.gso. now eauto.
-    intros Hc. subst. eapply Hnin.
-    now eexists; eauto.
-  Qed.
-
-  (** Extend the first environment with a list of variables in [Scope] *)
-  Lemma Fun_inv_set_lists_In_Scope_l k rho1 rho1' rho2 Scope Funs σ Γ xs vs :
-    Included _ (FromList xs) Scope ->
-    Fun_inv k rho1 rho2 Scope Funs σ Γ ->
-    set_lists xs vs rho1 = Some rho1' ->
-    Fun_inv k rho1' rho2 Scope Funs σ Γ.
-  Proof.
-    revert rho1 rho1' vs. induction xs; intros rho1 rho1' vs.
-    - intros Hinc Hfun Hset. inv Hset.
-      destruct vs; [ | discriminate ]. now inv H0.
-    - intros Hinc Hfun Hset.
-      simpl in Hset.
-      destruct vs; [ discriminate | ].
-      destruct (set_lists xs vs rho1) eqn:Heq; [ | discriminate ]. inv Hset.
-      eapply Fun_inv_set_In_Scope_l.
-      + rewrite FromList_cons in Hinc. 
-        eapply Hinc. eauto.
-      + eapply IHxs; eauto.
-        rewrite FromList_cons in Hinc. 
-        eapply Included_trans; [| eassumption ].
-        eapply Included_Union_r.
-  Qed.
-
-  (** Extend the second environment with a list of variables in [Scope] *)
-  Lemma Fun_inv_set_lists_In_Scope_r k rho1 rho2 rho2' Scope Funs σ Γ xs vs v :
-    Included _ (FromList xs) Scope ->
-    Disjoint _ (image σ (Setminus _ Funs Scope)) (FromList xs) ->
-    Fun_inv k rho1 (M.set Γ v rho2) Scope Funs σ Γ ->
-    set_lists xs vs rho2 = Some rho2' ->
-    Fun_inv k rho1 (M.set Γ v rho2') Scope Funs σ Γ.
-  Proof.
-    revert rho2 rho2' vs. induction xs; intros rho2 rho2' vs.
-    - intros Hinc Hd Hfun Hset. inv Hset.
-      destruct vs; [ | discriminate ]. now inv H0.
-    - intros Hinc Hd Hfun Hset.
-      simpl in Hset.
-      destruct vs; [ discriminate | ].
-      destruct (set_lists xs vs rho2) eqn:Heq; [ | discriminate ]. inv Hset.
-      eapply Fun_inv_set_In_Scope_r.
-      + rewrite FromList_cons in Hinc. 
-        eapply Hinc. eauto.
-      + intros Hin. eapply Hd. constructor; eauto.
-        rewrite FromList_cons. eauto.
-      + rewrite FromList_cons in Hinc, Hd. eapply IHxs; eauto.      
-        eapply Included_trans; [| eassumption ].
-        eapply Included_Union_r.
-        eapply Disjoint_Included_r; [| eassumption ].
-        eapply Included_Union_r.
-  Qed.
-
-  (** Redefine the environment argument in the second environment *)
-  Lemma Fun_inv_reset k rho rho' B v Scope Funs σ Γ :
-    ~ In _ (name_in_fundefs B) Γ ->
-    M.get Γ rho' = Some v ->
-    Fun_inv k rho (def_funs B B rho' rho') Scope Funs σ Γ ->
-    Fun_inv k rho (M.set Γ v (def_funs B B rho' rho')) Scope Funs σ Γ.
-  Proof. 
-    intros Hnin Hget Hinv f v1 Hninf Hinf Hget'.
-    edestruct Hinv with (f := f) as
-        [vs' [rho3 [B3 [f3 [rho4 [B4 [f4 [Hget1 [Heq2 [Ηnin2 [Hget2 Happrox]]]]]]]]]]]; eauto.
-    rewrite def_funs_neq in Hget1; eauto. subst.
-    repeat subst_exp.
-    repeat eexists; eauto.
-    now rewrite M.gss.
-    eapply def_funs_spec in Hget2. destruct Hget2 as [[Hname Heq] | [Hname Hget'']].
-    - inv Heq. rewrite M.gso.
-      rewrite def_funs_eq. reflexivity. eassumption.
-      intros Hc; subst; eauto.
-    - destruct (peq (σ f) Γ); subst.
-      rewrite M.gss. congruence.
-      rewrite M.gso.
-      rewrite def_funs_neq; eauto. 
-      now intros Hc; subst; eauto.
-  Qed.
-
-  Global Instance Fun_inv_proper :
-    Proper (Logic.eq ==> Logic.eq ==> Logic.eq ==> Same_set var ==>
-                     Logic.eq ==> Logic.eq ==> Logic.eq ==> iff)
-           (Fun_inv).
-  Proof.
-    constructor; intros Hinv; subst;
-    intros f v1 Hninf Hinf Hget;
-    edestruct Hinv with (f := f) as
-        [vs' [rho3 [B3 [f3 [rho4 [B4 [f4 [Hget1 [Heq2 [Ηnin2 [Hget2 Happrox]]]]]]]]]]]; eauto;
-    repeat eexists; try (now rewrite <- H2; eauto); try rewrite H2; eauto.
-  Qed.
-  
-  (** Define a block of functions in the first environment and put them in the
-    current scope *)
-  Lemma Fun_inv_def_funs_l k rho rho' B1 B1' Scope Funs σ Γ:
-    Disjoint _ (image σ (Setminus _ Funs Scope)) (name_in_fundefs B1') -> 
-    Fun_inv k rho rho' Scope Funs σ Γ ->
-    Fun_inv k (def_funs B1 B1' rho rho) rho'
-            (Union _ (name_in_fundefs B1')  Scope) Funs σ Γ.
-  Proof.
-    intros HD Hinv f v1 Hninf Hinf Hget. rewrite def_funs_neq in Hget; eauto.
-    edestruct Hinv with (f := f) as
-        [vs' [rho3 [B3 [f3 [rho4 [B4 [f4 [Hget1 [Heq2 [Ηnin2 [Hget2 Happrox]]]]]]]]]]]; eauto.
-    subst. repeat eexists; eauto.
-    intros Hc; inv Hc; eauto.
-    eapply HD. econstructor; eauto.
-    eexists; split; [| now eauto ]. constructor; eauto.
-  Qed.
-
-  (** Define a block of functions in the second environment and put the in the
-    current scope *)
-  Lemma Fun_inv_def_funs_r k rho rho' B1 B1' Scope Funs σ Γ:
-    ~ In _ (name_in_fundefs B1') Γ ->
-    Disjoint _ (image σ (Setminus _ Funs Scope)) (name_in_fundefs B1') -> 
-    Fun_inv k rho rho' Scope Funs σ Γ ->
-    Fun_inv k rho (def_funs B1 B1' rho' rho')
-            (Union _ (name_in_fundefs B1') Scope) Funs σ Γ.
-  Proof.
-    intros Hnin HD Hinv f v1 Hninf Hinf Hget.
-    edestruct Hinv with (f := f) as
-        [vs' [rho3 [B3 [f3 [rho4 [B4 [f4 [Hget1 [Heq2 [Ηnin2 [Hget2 Happrox]]]]]]]]]]]; eauto.
-    subst. repeat eexists; eauto.
-    now rewrite def_funs_neq; eauto.
-    intros Hc; inv Hc; eauto. 
-    eapply HD. econstructor; eauto. eexists;  split; [| now eauto ].
-    now constructor; eauto.
-    rewrite def_funs_neq; eauto. 
-    intros Hc. eapply HD. constructor; eauto. eexists; split; [| now eauto ].
-    now constructor; eauto.
-  Qed.
-
-  (** Define a block of functions in both environments and put the in the
-    current scope *)
-  Lemma Fun_inv_def_funs k rho rho' B1 B1' B2 B2' Scope Funs σ Γ:
-    ~ In _ (name_in_fundefs B2') Γ -> ~ In _ (name_in_fundefs B1') Γ ->
-    Disjoint _ (image σ (Setminus _ Funs Scope)) (name_in_fundefs B1') ->
-    Disjoint _ (image σ (Setminus _ Funs Scope)) (name_in_fundefs B2') ->
-    Fun_inv k rho rho' Scope Funs σ Γ ->
-    Fun_inv k  (def_funs B1 B1' rho rho) (def_funs B2 B2' rho' rho')
-            (Union _ (name_in_fundefs B1') Scope) Funs σ Γ.
-  Proof.
-    intros Hnin1 Hnin2 HD1 HD2 Hinv f v1 Hninf Hinf Hget.
-    rewrite def_funs_neq in Hget; eauto.
-    edestruct Hinv with (f := f) as
-        [vs' [rho3 [B3 [f3 [rho4 [B4 [f4 [Hget1 [Heq2 [Ηnin2 [Hget2 Happrox]]]]]]]]]]]; eauto.
-    subst. repeat eexists; eauto.
-    now rewrite def_funs_neq; eauto.
-    intros Hc; inv Hc; eauto.
-    eapply HD1. econstructor; eauto. eexists; split; [| now eauto ].
-    now constructor; eauto.
-    rewrite def_funs_neq; eauto.
-    intros Hc. eapply HD2. econstructor; eauto. eexists; split; [| now eauto ].
-    now constructor; eauto.
-  Qed.
-  
-  (** * Lemmas about FV_inv *)
-
-  (** Extend the first environment with a variable in [Scope] *)
-  Lemma FV_inv_set_In_Scope_l k rho rho' x v Scope Funs GFuns FVs c Γ :
-    In var Scope x ->
-    FV_inv k rho rho' Scope Funs GFuns c Γ FVs ->
-    FV_inv k (M.set x v rho) rho' Scope Funs GFuns c Γ FVs.
-  Proof.
-    intros Hin [g [c' [Hget [Hleq HInv]]]].
-    destruct FVs.
-    - inv HInv. exists g.
-      eexists; repeat split; eauto.
-    - do 2 eexists; repeat split; eauto.
-      rewrite <- Hleq; eauto. congruence.
-      eapply Forall2_monotonic_strong; [| eassumption ].
-      intros z w Hin1 Hin2 He v1 Hnin1 Hnin2 Hnin3 Hget'.
-      eapply He; eauto. rewrite M.gso in Hget'; eauto.
-      intros Hc; subst; contradiction. 
-  Qed.
-  
-  (** Extend the first environment with a variable not in [FVs] *)
-  Lemma FV_inv_set_not_In_FVs_l k rho rho' x v Scope Funs GFuns c Γ FVs :
-    ~ List.In x FVs ->
-    FV_inv k rho rho' Scope Funs GFuns c Γ FVs ->
-    FV_inv k (M.set x v rho) rho' Scope Funs GFuns c Γ FVs.
-  Proof.
-    intros Hnin [c' [g [Hget [Hleq HInv]]]].
-    destruct FVs.
-    - inv HInv. exists c'.
-      eexists; repeat split; eauto.
-    - do 2 eexists; repeat split; eauto.
-      rewrite <- Hleq; eauto. congruence.
-      eapply Forall2_monotonic_strong; [| eassumption ].
-      intros z w Hin1 Hin2 He v1 Hnin1 Hnin2 Hnin3 Hget'.
-      eapply He; eauto. rewrite M.gso in Hget'; eauto.
-      intros Hc; subst; contradiction. 
-  Qed.
-  
-  (** Extend the second environment with a variable that is not [Γ] *)
-  Lemma FV_inv_set_r k rho rho' x v Scope Funs GFuns c Γ FVs :
-    x <> Γ ->
-    FV_inv k rho rho' Scope Funs GFuns c Γ FVs ->
-    FV_inv k rho (M.set x v rho') Scope Funs GFuns c Γ FVs.
-  Proof.
-    intros Hnin [c' [g [Hget HInv]]]. do 2 eexists; split; eauto.
-    rewrite M.gso; eauto.
-  Qed.
-
-
-  (** Extend the [Scope] and remove from [GFuns] **)
-  Lemma FV_inv_extend_Scope_GFuns k rho rho' Scope GFuns Funs c Γ FVs x :
-    FV_inv k rho rho' Scope Funs GFuns c Γ FVs ->
-    FV_inv k rho rho' (x |: Scope) Funs (GFuns \\ [set x]) c Γ FVs.
-  Proof.
-    intros [c' [g [Hget [Hc HInv]]]]. do 2 eexists; split; eauto.
-    split; eauto.
-    eapply Forall2_monotonic_strong; [| eassumption ]; eauto.
-    intros; eauto. eapply H1; eauto.
-    intros Hc'; eapply H4. constructor; eauto.  
-  Qed.
-
-  Lemma FV_inv_monotonic k j rho rho' Scope GFuns Funs c Γ FVs :
-    FV_inv j rho rho' Scope Funs GFuns c Γ FVs ->
-    j >= k ->
-    FV_inv k rho rho' Scope Funs GFuns c Γ FVs.
-  Proof.
-    intros [c' [g [Hget [Hc HInv]]]]. do 2 eexists; split; eauto.
-    split; eauto.
-    eapply Forall2_monotonic_strong; [| eassumption ]; eauto.
-    intros; eauto. eapply cc_approx_val_monotonic. eauto. eassumption.
-  Qed.
-
-  Lemma FV_inv_antimonotonic_GFuns k rho rho' Scope GFuns1 GFuns2 Funs c Γ FVs :
-    FV_inv k rho rho' Scope Funs GFuns1 c Γ FVs ->
-    GFuns1 \subset GFuns2 ->
-    FV_inv k rho rho' Scope Funs GFuns2 c Γ FVs.
-  Proof.
-    intros [c' [g [Hget [Hc HInv]]]]. do 2 eexists; split; eauto.
-    split; eauto.
-    eapply Forall2_monotonic_strong; [| eassumption ]; eauto.
-  Qed.
-  
-  Lemma FV_inv_antimonotonic_add_global_funs k rho rho' Scope GFuns GFuns' names {Hd : Decidable names} Funs c Γ FVs FVs' :
-    FV_inv k rho rho' Scope Funs GFuns c Γ FVs ->
-    add_global_funs GFuns names (FromList FVs') GFuns' ->
-    names \subset Scope ->
-    FV_inv k rho rho' Scope Funs GFuns' c Γ FVs.
-  Proof.
-    intros [c' [g [Hget [Hc HInv]]]] Hadd Hsub. inv Hadd; eauto.
-    - do 2 eexists; split; eauto.
-      split; eauto.
-      eapply Forall2_monotonic_strong; [| eassumption ]; eauto.
-    - do 2 eexists; split; eauto.
-      split; eauto.
-      eapply Forall2_monotonic_strong; [| eassumption ]; eauto.
-      intros. eapply H2; eauto.    
-      destruct Hd. destruct (Dec x1); eauto. intros Hc1.
-      eapply H5. constructor; eauto. 
-  Qed.
-
-  Lemma FV_inv_Forall2 k rho rho' Scope GFuns Funs c Γ FVs vs1 vs2 :
-    get_list FVs rho = Some vs1 ->
-    M.get Γ rho' = Some (Vconstr c vs2) ->
-    Forall2 (cc_approx_val pr cenv clo_tag k boundG) vs1 vs2 ->
-    FV_inv k rho rho' Scope Funs GFuns c Γ FVs.
-  Proof.
-    intros Hget1 Hget2 Hall. do 2 eexists; split; eauto. 
-    split; eauto. clear Hget2.
-    revert vs1 vs2 Hget1 Hall; induction FVs; intros vs1 vs2 Hget1 Hall;
-      destruct vs2; try (now inv Hget1).
-    + inv Hall; eauto.
-      eapply get_list_length_eq in Hget1. simpl in Hget1. congruence.
-    + inv Hall.
-      constructor; eauto.
-      * intros. simpl in Hget1.
-        rewrite H4 in Hget1.
-        destruct (get_list FVs rho) eqn:Hfv; try congruence.
-      * simpl in Hget1.
-        destruct (get_list FVs rho) eqn:Hfv; try congruence; destruct (M.get a rho); try congruence. 
-        inv Hget1. eapply IHFVs; eauto.
-  Qed.
-
-  (** Extend the [Scope]. TODO : replace with monotonicity property? *)
-  Lemma FV_inv_extend_Scope k rho rho' Scope GFuns Funs c Γ FVs x :
-    FV_inv k rho rho' Scope Funs GFuns c Γ FVs ->
-    FV_inv k rho rho' (Union _ (Singleton _ x) Scope) Funs GFuns c Γ FVs.
-  Proof.
-    intros [c' [g [Hget [Hc HInv]]]]. do 2 eexists; split; eauto.
-    split; eauto.
-    eapply Forall2_monotonic_strong; [| eassumption ]; eauto.
-  Qed.
-  
-  (** Define a block of functions in both environments and put the in the
-    current scope *)
-  Lemma FV_inv_def_funs k rho rho' B1 B1' B2 B2' Scope Funs GFuns c Γ FVs:
-    ~ In _ (name_in_fundefs B1') Γ ->
-    ~ In _ (name_in_fundefs B2') Γ ->
-    FV_inv k rho rho' Scope Funs GFuns c Γ FVs ->
-    FV_inv k  (def_funs B1 B1' rho rho) (def_funs B2 B2' rho' rho')
-           (Union _ (name_in_fundefs B1') Scope) Funs GFuns c Γ FVs.
-  Proof.
-    intros Hnin1 Hnin2 [c' [g [Hget [Hc HInv]]]]. do 2 eexists; split; eauto.
-    now rewrite def_funs_neq; eauto.    
-    split; eauto.
-    eapply Forall2_monotonic_strong; [| eassumption ]; eauto.
-    intros z w Hin1 Hin2 He v1 Hnin3 Hnin4 Hnin5 Hget'.
-    eapply He; eauto. now rewrite def_funs_neq in Hget'; eauto.
-  Qed.
-
-  (** * Lemmas about [GFun_inv]  *)
-
-  (** Extend the two environments with a variable that is not the current environment
-    argument (i.e. [Γ]) *)
-  Lemma GFun_inv_set k rho rho' Scope GFuns σ f rho1 B1 f1 rho2 B2 f2:
-    GFun_inv k rho rho' Scope (GFuns \\ [set f]) σ ->
-    ~ In _ Scope (σ f) ->
-    ~ In _ (image σ (GFuns \\ [set f])) (σ f) ->
-    (forall c, f \in GFuns ->
-          cc_approx_val pr cenv clo_tag k boundG (Vfun rho1 B1 f1) (Vconstr clo_tag [(Vfun rho2 B2 f2) ; Vconstr c []])) ->
-    GFun_inv k (M.set f (Vfun rho1 B1 f1) rho) (M.set (σ f) (Vfun rho2 B2 f2) rho') Scope GFuns σ.
-  Proof.
-    intros Hinv Hnin Hnin' Hv f'' v Hnin'' Hin Hget'.
-    destruct (peq f'' f); subst; eauto.
-    - rewrite M.gss in Hget'. inv Hget'. repeat eexists; eauto.
-      now rewrite M.gss.
-    - rewrite M.gso in Hget'; eauto.
-      edestruct Hinv with (f0 := f'') as
-          [rho3 [B3 [f3 [rho4 [B4 [f4 [Heq [Ηnin2 [Hget2 Happrox]]]]]]]]]; subst; eauto.
-      constructor; eauto. intros Hc. inv Hc. congruence. repeat eexists; eauto.
-      rewrite M.gso. now eauto. 
-      intros Hc. eapply Hnin'. rewrite <- Hc. eapply In_image. constructor; eauto.
-      intros Hc'. inv Hc'. contradiction.
-  Qed.
-  
-  (** Extend the first environment with a variable not in [GFuns] *)
-  Lemma GFun_inv_set_not_In_GFuns_l k rho1 rho2 Scope GFuns σ x v :
-    ~ x \in GFuns ->
-    GFun_inv k rho1 rho2 Scope GFuns σ ->
-    GFun_inv k (M.set x v rho1) rho2 Scope GFuns σ.
-  Proof.
-    intros Hnin Hinv f v' c Hin Hget.
-    eapply Hinv; eauto. rewrite M.gso in Hget.
-    now eauto. intros Hc; subst. now eauto.
-  Qed.
-
-  (** Extend the second environment with a variable in [GFuns] *)
-  Lemma GFun_inv_set_not_In_GFuns_r k rho1 rho2 Scope GFuns σ x v :
-    ~ x \in (image σ GFuns) ->
-    GFun_inv k rho1 rho2 Scope GFuns σ ->
-    GFun_inv k rho1 (M.set x v rho2) Scope GFuns σ.
-  Proof.
-    intros Hnin Hinv f v' c Hin Hget.
-    edestruct Hinv as
-        [rho3 [B3 [f3 [rho4 [B4 [f4 [Heq2 [Ηnin2 [Hget2 Happrox]]]]]]]]]; eauto.
-    repeat eexists; eauto.
-    rewrite M.gso. eassumption.
-    intros Hc. eapply Hnin. subst. eapply In_image. eassumption. 
-  Qed.
-
-  (** Extend the first environment with a variable not in [GFuns] *)
-  Lemma GFun_inv_setlist_not_In_GFuns_l k rho1 rho1' rho2 Scope GFuns σ xs vs :
-    Disjoint _ (FromList xs) GFuns ->
-    set_lists xs vs rho1 = Some rho1' ->
-    GFun_inv k rho1 rho2 Scope GFuns σ ->
-    GFun_inv k rho1' rho2 Scope GFuns σ.
-  Proof.
-    revert rho1 rho1' vs. induction xs; intros rho1 rho1' vs.
-    - intros Hinc Hset Hfun. inv Hset.
-      destruct vs; [ | discriminate ]. now inv H0.
-    - intros Hinc Hset Hfun.
-      simpl in Hset.
-      destruct vs; [ discriminate | ].
-      destruct (set_lists xs vs rho1) eqn:Heq; [ | discriminate ]. inv Hset.
-      eapply GFun_inv_set_not_In_GFuns_l.
-      + intros Hc; eapply Hinc. constructor; eauto.
-        now left.
-      + eapply IHxs; eauto.
-        eapply Disjoint_Included_l; [| eassumption ].
-        rewrite FromList_cons; sets.
-  Qed.
-
-  (** Extend the second environment with a list not in [GFuns] *)
-  Lemma GFun_inv_setlist_not_In_GFuns_r k rho1 rho2' rho2 Scope GFuns σ xs vs :
-    Disjoint _ (FromList xs) (image σ GFuns) ->
-    set_lists xs vs rho2 = Some rho2' ->
-    GFun_inv k rho1 rho2 Scope GFuns σ ->
-    GFun_inv k rho1 rho2' Scope GFuns σ.
-  Proof.
-    revert rho2 rho2' vs. induction xs; intros rho2 rho2' vs.
-    - intros Hinc Hset Hfun. inv Hset.
-      destruct vs; [ | discriminate ]. now inv H0.
-    - intros Hinc Hset Hfun.
-      simpl in Hset.
-      destruct vs; [ discriminate | ].
-      destruct (set_lists xs vs rho2) eqn:Heq; [ | discriminate ]. inv Hset.
-      eapply GFun_inv_set_not_In_GFuns_r.
-      + intros Hc; eapply Hinc. constructor; eauto.
-        now left.
-      + eapply IHxs; eauto.
-        eapply Disjoint_Included_l; [| eassumption ].
-        rewrite FromList_cons; sets.
-  Qed.
-
-  (** Extend the first environment with funs not in [GFuns] *)
-  Lemma GFun_inv_def_funs_not_In_GFuns_l k rho1 rho2 Scope GFuns σ B1 B1' :
-    Disjoint _ (name_in_fundefs B1') GFuns ->
-    GFun_inv k rho1 rho2 Scope GFuns σ ->
-    GFun_inv k (def_funs B1 B1' rho1 rho1) rho2 Scope GFuns σ.
-  Proof.
-    intros HD Hinv f v1 c Hinf Hget. rewrite def_funs_neq in Hget; eauto.
-    intros Hc. eapply HD. constructor; eauto.
-  Qed.
-
-  Lemma GFun_inv_def_funs_not_In_GFuns_r k rho rho' B1 B1' Scope GFuns σ :
-    Disjoint _ (image σ GFuns) (name_in_fundefs B1') ->
-    GFun_inv k rho rho' Scope GFuns σ ->
-    GFun_inv k rho (def_funs B1 B1' rho' rho') Scope GFuns σ.
-  Proof.
-    intros HD Hinv f v1 c Hinf Hget. setoid_rewrite def_funs_neq; eauto.
-    intros Hc. eapply HD. constructor; sets.
-  Qed.
-
-  Lemma GFun_inv_antimon k rho rho' Scope GFuns GFuns' σ :
-     GFun_inv k rho rho' Scope GFuns σ ->
-     GFuns' \subset GFuns ->
-     GFun_inv k rho rho' Scope GFuns' σ .
-  Proof.
-    intros Hg Hsub f v1 Hinf Hget; eauto.
-  Qed.
-
-  Lemma GFun_inv_Scope k rho rho' Scope Scope' GFuns σ :
-    Disjoint _ Scope' (image σ GFuns) -> 
-    GFun_inv k rho rho' Scope GFuns σ ->
-    GFun_inv k rho rho' Scope' GFuns σ.
-  Proof.
-    intros Hd Hg f v1 c Hinf Hget; eauto.
-    edestruct Hg as (rho1 & B1 & f1 & rho2 & B2 & f2 & Heq1 & Hnin & Hget1 & Hcc); eauto.
-    repeat eexists; eauto.
-    intros Hc. eapply Hd. constructor; eauto.
-    eapply In_image. eassumption.
-  Qed. 
-
-  Lemma GFun_inv_monotonic k j rho rho' Scope GFuns σ :
-    GFun_inv k rho rho' Scope GFuns σ ->
-    j <= k ->
-    GFun_inv j rho rho' Scope GFuns σ.
-  Proof.
-    intros Hg Hleq c f v1 Hinf Hget; eauto.
-    edestruct Hg as (rho1 & B1 & f1 & rho2 & B2 & f2 & Heq1 & Hnin & Hget1 & Hcc); eauto.
-    repeat eexists; eauto.
-    eapply cc_approx_val_monotonic; eauto.
-  Qed.
-  
-  Lemma GFun_inv_Scope_extend k rho rho' Scope Scope' GFuns σ :
-    Disjoint _ (image σ GFuns) Scope' ->
-    GFun_inv k rho rho' Scope GFuns σ ->
-    GFun_inv k rho rho' (Scope' :|: Scope) GFuns σ.
-  Proof.
-    intros Hdis Hg f v1 c1 Hinf Hget; eauto.
-    edestruct Hg as (rho1 & B1 & f1 & rho2 & B2 & f2 & Heq & Hnin & Hget' & Hcc); eauto.
-    subst. repeat eexists; eauto.
-    intros Hc. inv Hc; eauto.
-    eapply Hdis. constructor; eauto.
-    now eapply In_image. 
-  Qed.
-
-  Lemma GFun_inv_fuse k rho rho' Scope1 Scope2 GFuns1 GFuns2 σ names FVs { Hd : Decidable names} :
-    add_global_funs GFuns1 names FVs GFuns2 ->
-    GFun_inv k rho rho' Scope1 (GFuns1 \\ names) σ ->
-    GFun_inv k rho rho' Scope2 GFuns2 σ ->
-    Scope2 \subset Scope1 ->
-    Disjoint _ Scope1 (image σ names) ->
-    GFun_inv k rho rho' Scope1 GFuns2 σ.
-  Proof.
-    intros Ha Hg1 Hg2 Hsub Hd' x v c Hin1 Hget. inv Ha.
-    - destruct Hd. destruct (Dec x); eauto.
-      * edestruct Hg2 as (rho1 & B1 & f1 & rho2 & B2 & f2 & Heq1 & Hnin & Hget1 & Hcc); eauto.
-        repeat eexists; eauto.
-        intros Hc. eapply Hd'. constructor; eauto.
-        eapply In_image. eassumption.
-      * inv Hin1; try contradiction.  
-        edestruct Hg1 as (rho1 & B1 & f1 & rho2 & B2 & f2 & Heq1 & Hnin & Hget1 & Hcc); eauto.
-        constructor; eauto.
-        repeat eexists; eauto.
-    - eauto.
-  Qed.
-
-  Lemma Fun_inv_from_GFun_inv k rho1 rho2 Scope GFuns Funs σ Γ c :
-    Funs \subset GFuns -> 
-    GFun_inv k rho1 rho2 Scope (GFuns \\ Scope) σ ->
-    M.get Γ rho2 = Some (Vconstr c []) ->  
-    Fun_inv k rho1 rho2 Scope Funs σ Γ.
-  Proof.
-    intros Hsub Hinv Hget f v' Hnin Hin Hget'.
-    edestruct Hinv as
-        [rho3 [B3 [f3 [rho4 [B4 [f4 [Heq2 [Ηnin2 [Hget2 Happrox]]]]]]]]]; eauto.
-    now constructor; eauto. 
-    repeat eexists; eauto.
-  Qed.
   
   (** * Lemmas about the existance of the interpretation of an evaluation context *)
   
@@ -946,64 +155,6 @@ Section Closure_conversion_correct.
         intros Hin. eapply HD. now eauto.
       + eassumption.
       + exists rho2''. eapply ctx_to_rho_comp_ctx_f_r; eassumption.
-  Qed.
-
-  Lemma add_global_funs_included G F {_ : Decidable F} V G' :
-    add_global_funs G F V G' ->
-    G \subset G' :|: F.
-  Proof. 
-    intros Hin. inv Hin; sets.
-  Qed.
-  
-  Lemma add_global_funs_included_r G F V G' :
-    add_global_funs G F V G' ->
-    G' \subset G :|: F.
-  Proof. 
-    intros Hin. inv Hin; sets.
-  Qed.
-
-  Definition is_gfuns (GFuns : Ensemble var) names (FVs : list var) GFuns' :=
-    (FVs = [] /\ GFuns' \subset GFuns :|: names) \/
-    (FVs <> [] /\ GFuns' \subset GFuns \\ names).
-
-  Lemma add_global_funs_is_gfuns (GFuns : Ensemble var) names (FVs : list var) GFuns':
-    add_global_funs GFuns names (FromList FVs) GFuns' ->
-    is_gfuns GFuns names FVs GFuns'.
-  Proof.
-    intros Hin; destruct FVs; inv Hin; unfold is_gfuns; sets.
-    - exfalso. eapply not_In_Empty_set. eapply H.
-      now left.
-    - right. split; sets. congruence.
-  Qed.
-
-  Lemma is_gfuns_setminus (GFuns : Ensemble var) names (FVs : list var) GFuns' x:
-   is_gfuns GFuns (x |: names) FVs GFuns' ->
-   is_gfuns GFuns names FVs (GFuns' \\ [set x]).
-  Proof.
-    intros [[H1 H2] | [H1 H2]]; subst; unfold is_gfuns in *.
-    left; split; eauto.
-    eapply Setminus_Included_Included_Union. eapply Included_trans. eassumption. sets.
-    right; split; eauto.
-    eapply Setminus_Included_Included_Union. eapply Included_trans. eassumption. sets.
-  Qed.
-
-  Lemma is_gfuns_included_r G F {_ : Decidable F} V G' :
-    is_gfuns G F V G' ->
-    G' \subset G :|: F.
-  Proof. 
-    intros Hin. destruct Hin as [[? ?] | [? ?]]; subst; sets.
-    eapply Included_trans. eassumption. sets.
-  Qed.
-
-  Lemma add_global_funs_is_gfuns_included (GFuns : Ensemble var) names (FVs : list var) GFuns' GFuns'' :
-    add_global_funs GFuns names (FromList FVs) GFuns' ->
-    is_gfuns GFuns names FVs GFuns'' ->
-    GFuns'' \subset GFuns'.
-  Proof.
-    intros Hadd Hin; destruct Hin as [[? ?] | [? ?]]; inv Hadd; unfold is_gfuns; sets.
-    - eapply Included_trans. eassumption. sets.
-    - rewrite FromList_nil in H1. exfalso; eapply H1; reflexivity.
-    - eapply Included_trans. eassumption. sets.
   Qed.
 
   (** * Correctness lemmas *)
@@ -1436,6 +587,7 @@ Section Closure_conversion_correct.
   Qed.
   
 
+
   (** Correctness of [make_closures] *)
   Lemma make_closures_correct k rho1 rho2 rho2' B S Γ' C σ S' Scope Funs GFuns FVs c Γ :
     make_closures clo_tag B S Γ' C σ S' ->
@@ -1860,6 +1012,234 @@ Section Closure_conversion_correct.
         eapply le_trans; [| eapply plus_le_compat_r; eapply mult_le_compat_l; now apply max_exp_env_Eproj ].
         simpl. omega. }
     - (* Case letapp *)
+      inv Hcc. intros v1 c2 Hleq Hstep.
+      assert (Hstep' := Hstep). inv Hstep'.
+      
+      assert (Hadm : sizeOf_exp_ctx C <= 4 + 4 * length ys).
+      { eapply le_trans. eapply project_vars_sizeOf_ctx_exp; eauto. simpl; omega. }
+      
+      pose (P :=
+              fun n c1 c2 : nat =>
+                c1 + n <= c2 + sizeOf_exp_ctx C <= 8 * c1 * max_exp_env k e rho1
+                                                 + 8 * sizeOf_exp e + n).
+      edestruct project_vars_ctx_to_rho as [rho2' Hto_rho]; eauto.
+      simpl. rewrite H5, H7. reflexivity. 
+      edestruct project_vars_correct as [Happ [Hfun' [Hgfun' [Henv' Hvar]]]]; eauto. 
+      edestruct Hvar as [v' [Hget' Happ']]; eauto.
+      simpl. rewrite H5, H7. reflexivity.
+      simpl in Hget'.
+      destruct (M.get f' rho2') eqn:Hgetf';
+        destruct (get_list ys' rho2') eqn:Hgetvs; try congruence. inv Hget'. 
+      inv Happ'.
+      assert (Hv := H2). rewrite cc_approx_val_eq in H2.
+      destruct v0 as [ | | ]; try contradiction.
+      simpl in H2. destruct l0 as [ | ? [|]] ; try contradiction; destruct v0;  try contradiction.      
+      destruct v2; try contradiction.
+      edestruct H2 as [Gamma [xs2 [e2' [rho2'' [Heqc [Hfdef [Hset Hlt]]]]]]]; [ | now eauto | now eauto | ].
+      eapply Forall2_length. eassumption.
+      subst.
+
+      eapply cc_approx_exp_rel_mon with (P1 := P (sizeOf_exp_ctx C)).
+      { eapply ctx_to_rho_cc_approx_exp with (P' := P 0).
+        - now firstorder.
+        - clear; firstorder.
+        - eassumption.
+        - eapply cc_approx_exp_letapp_compat with (P' := boundL k e rho1) (rho1 := rho1) (f1 := f).
+          + admit. (* bound *)
+          + admit.
+          + admit.
+          + intros v3 v4. repeat subst_exp. eexists; split; eauto.
+          + eapply Forall2_cc_approx_var_env; eauto.
+          + econstructor. eassumption. reflexivity. econstructor. 
+            rewrite M.gso. eassumption. admit.
+            reflexivity. now constructor.
+          + intros m v4 v5 Hleq' Hvs. 
+            eapply IHe; [ | | | | | | | | | eassumption ].
+            * eapply cc_approx_env_P_extend.
+              eapply cc_approx_env_P_antimon; [ eassumption |]...
+              eassumption.
+            * now eauto.
+            * eapply binding_in_map_antimon; [| eapply binding_in_map_set; eassumption ].
+              eapply occurs_free_Eproj_Included.
+            * intros f Hfin. eauto.
+            * eapply injective_subdomain_antimon; eauto; sets.
+            * eapply Disjoint_Included_r;
+              [| eapply Disjoint_Included_l; [ apply image_monotonic | now apply Hd ]].
+              normalize_bound_var... now eauto with Ensembles_DB.
+            * eapply Fun_inv_set_In_Scope_l. now eauto.
+              eapply Fun_inv_set_In_Scope_r_not_Γ. now eauto.
+              intros Heq; subst. now eauto.
+              eapply Fun_inv_mon; [ | now eauto ].
+              eapply Disjoint_Included; [ | | now apply Hd ].
+              normalize_bound_var... sets.
+            * eapply FV_inv_set_In_Scope_l. now constructor.
+              eapply FV_inv_set_r. intros Hc. eapply Hnin.
+              subst. now eauto. now eapply FV_inv_extend_Scope_GFuns.
+            * eapply GFun_inv_set_not_In_GFuns_l.
+              now intros Hc; inv Hc; eauto.
+              eapply GFun_inv_set_not_In_GFuns_r.
+              intros Hc. eapply Hd. constructor.
+              rewrite image_Union. right. eapply image_monotonic; eauto...
+              normalize_bound_var... sets.
+              eapply GFun_inv_Scope_extend; sets.
+              eapply Disjoint_Included; [| | now eapply Hd ].
+              normalize_bound_var... sets.
+              eapply GFun_inv_antimon; sets. }
+
+            rewrite (Union_commut [set f']), <- Union_assoc.
+            intros Hc. inv Hc; eauto. now inv H1; eauto.
+            
+            inv H2; eauto.
+          unfold P.
+          unfold boundL, upper_boundL, lower_boundL, P. intros c1 c2.
+          rewrite <- !plus_n_O. intros [Hle1 Hle2]; split; try omega.
+          ring_simplify. omega. rewrite <- !plus_assoc.
+            rewrite (plus_comm _ (8 * _)), (plus_assoc _ (8 * _)).
+            eapply plus_le_compat; eauto.
+            eapply le_trans with (m := 5). omega.
+            specialize (max_exp_env_grt_1 k e rho1). omega.
+          now firstorder.
+        - clear; now firstorder.
+        -
+
+          
+      (*     + eassumption. *)
+      (*     + unfold boundL, upper_boundL, lower_boundL, P. intros c1 c2. *)
+      (*       rewrite <- !plus_n_O. intros [Hle1 Hle2]; split; try omega. *)
+      (*       ring_simplify.  rewrite <- !plus_assoc. *)
+      (*       rewrite (plus_comm _ (8 * _)), (plus_assoc _ (8 * _)). *)
+      (*       eapply plus_le_compat; eauto. *)
+      (*       eapply le_trans with (m := 5). omega. *)
+      (*       specialize (max_exp_env_grt_1 k e rho1). omega. *)
+      (*     + intros v1' v2' c1 vs1 Hget Hin Hv. *)
+      (*       unfold boundL, lower_boundL, upper_boundL, max_exp_env. *)
+      (*       erewrite <- sizeOf_env_set_proj; eauto. *)
+      (* { intros c1 c2. unfold P, boundL, lower_boundL, upper_boundL. *)
+      (*   intros [Hle1 Hle2]; split; try omega. *)
+      (*   eapply le_trans; [| eapply plus_le_compat_r; eapply mult_le_compat_l; now apply max_exp_env_Eproj ]. *)
+      (*   simpl. omega. } *)
+      
+      (* assert(Hadm : sizeOf_exp_ctx C <= 4 * length l + 4) *)
+      (*   by (eapply le_trans; [ now eapply project_vars_sizeOf_ctx_exp; eauto | simpl; omega ]). *)
+      (* pose (P := *)
+      (*         fun n c1 c2 : nat => *)
+      (*           c1 + n <= c2 + sizeOf_exp_ctx C <= 8 * c1 * max_exp_env k (Eapp v t l) rho1 *)
+      (*                                            + 8 * sizeOf_exp (Eapp v t l)  *)
+      (*                                            + n). *)
+      (* eapply cc_approx_exp_rel_mon with (P1 := P (sizeOf_exp_ctx C)); *)
+      (*   [| intros n1 n2; unfold P, boundL, upper_boundL, lower_boundL; simpl; omega ]. *)
+      (* { intros v1 c1 Hleq Hstep. assert (Hstep' := Hstep); inv Hstep'. *)
+      (*   simpl. rewrite H4, H5. reflexivity. *)
+      (*   simpl in Hget'. destruct (M.get f' rho2') eqn:Hgetf'; try discriminate. *)
+      (*   destruct (get_list ys' rho2') eqn:Hget_list'; try discriminate. inv Hget'. *)
+      (*   inv Happ'. rewrite cc_approx_val_eq in H6. destruct v0; try contradiction. *)
+      (*   eapply ctx_to_rho_cc_approx_exp with (P' := P 0); *)
+      (*     [ now firstorder *)
+      (*     | now (intros n1 n2; simpl; unfold P; intros; omega) | | | | ]; try eassumption. *)
+      (*   intros v1' c1' Hleq' Hstep'. inv Hstep'. repeat subst_exp. *)
+      (*   destruct l1; try contradiction. destruct v0, l1; try contradiction. *)
+      (*   destruct v2; try contradiction. eapply bstep_cost_deterministic in H21. *)
+      (*   2:eapply H12. inv H21. *)
+      (*   assert (Hlen := List_util.Forall2_length _ _ _ H9). *)
+      (*   edestruct H6 with (vs2 := l0) (j := k - 1) *)
+      (*     as [Γ' [xs2 [e2 [rho2'' [Heq [Hfind [Hset Hyp]]]]]]]; eauto. *)
+      (*   edestruct Hyp with (c1:=c1) as [v2' [c'2 [Hstep2 [[Hle1 Hle2] Hcc']]]]; try eassumption. *)
+      (*   - omega. *)
+      (*   - eapply List_util.Forall2_monotonic; [| eassumption ]. *)
+      (*     intros. eapply cc_approx_val_monotonic. eassumption. omega. *)
+      (*   - omega.           *)
+      (*   - subst. *)
+      (*     assert (Heq: length ys' = length l). *)
+      (*     { symmetry. do 2 (erewrite get_list_length_eq; [| eassumption ]). *)
+      (*       eapply Forall2_length. eassumption. }  *)
+      (*     repeat eexists. *)
+      (*     + econstructor. eassumption. reflexivity. *)
+      (*       econstructor. rewrite M.gso. eassumption.  *)
+      (*       intros Hc; subst.   *)
+      (*       eapply project_vars_not_In_free_set; [ eassumption | | ]. *)
+      (*       eassumption. eauto. constructor. now eapply H11. now left. *)
+      (*       reflexivity. *)
+      (*       eapply BStepc_app. rewrite M.gso. rewrite M.gss. reflexivity. *)
+      (*       now eauto. *)
+      (*       simpl. rewrite M.gss. rewrite get_list_set_neq. rewrite get_list_set_neq. *)
+      (*       rewrite Hget_list'. reflexivity.  *)
+      (*       intros Hin. eapply project_vars_not_In_free_set. eassumption. eassumption.  *)
+      (*       constructor. eapply H11. rewrite FromList_cons. now eauto. *)
+      (*       intros Hin. eapply project_vars_not_In_free_set. eassumption. eassumption. *)
+      (*       constructor. now eauto. rewrite FromList_cons. now eauto. *)
+      (*       eassumption. simpl in Hset. eauto. eassumption.  *)
+      (*     + simpl. unfold boundG, boundL, upper_boundL, lower_boundL in Hle1. *)
+      (*       omega. *)
+      (*     + unfold boundG, boundL, upper_boundL, lower_boundL in Hle2. *)
+      (*       assert (Hles : sizeOf_exp e0 <= sizeOf_env k rho1). *)
+      (*       { eapply le_trans; [| now eapply sizeOf_env_get; eauto ]. *)
+      (*         destruct k; try omega. simpl. eapply le_trans.  *)
+      (*         eapply fun_in_fundefs_sizeOf_exp; eauto. now eapply find_def_correct; eauto. *)
+      (*         now apply Max.le_max_l. } *)
+      (*       rewrite <- ! plus_assoc. rewrite <- plus_n_O. *)
+      (*       eapply plus_le_compat; [| simpl; omega ]. *)
+      (*       rewrite <- mult_assoc, NPeano.Nat.mul_add_distr_r, NPeano.Nat.mul_add_distr_l. *)
+      (*       eapply le_trans. eassumption. eapply plus_le_compat. *)
+      (*       { destruct (Nat.eq_0_gt_0_cases k); subst. *)
+      (*         * unfold max_exp_env. rewrite sizeOf_env_O, Max.max_0_r. *)
+      (*           rewrite mult_assoc. eapply mult_le_compat_l. *)
+      (*           eapply le_trans. eassumption. now apply Max.le_max_r. *)
+      (*         * eapply le_trans. eapply mult_le_compat_l. *)
+      (*           eapply sizeOf_env_set_app; eauto. *)
+      (*           eapply fun_in_fundefs_sizeOf_exp; eauto. now eapply find_def_correct; eauto. *)
+      (*           rewrite mult_assoc. eapply mult_le_compat_l. now apply Max.le_max_r. } *)
+      (*       { rewrite mult_assoc. eapply mult_le_compat. omega. *)
+      (*         eapply le_trans; [eassumption |  now apply Max.le_max_r ]. } *)
+      (*     + eapply cc_approx_val_monotonic. eassumption. omega. } *)
+
+      (*     eapply ctx_to_rho_cc_approx_exp with (P' := P 2). *)
+      (*     eapply cc_approx_exp_proj_compat with (S0 := boundL k e rho1). *)
+      (*     + eassumption. *)
+      (*     + unfold boundL, upper_boundL, lower_boundL, P. intros c1 c2. *)
+      (*       rewrite <- !plus_n_O. intros [Hle1 Hle2]; split; try omega. *)
+      (*       ring_simplify.  rewrite <- !plus_assoc. *)
+      (*       rewrite (plus_comm _ (8 * _)), (plus_assoc _ (8 * _)). *)
+      (*       eapply plus_le_compat; eauto. *)
+      (*       eapply le_trans with (m := 5). omega. *)
+      (*       specialize (max_exp_env_grt_1 k e rho1). omega. *)
+      (*     + intros v1' v2' c1 vs1 Hget Hin Hv. *)
+      (*       unfold boundL, lower_boundL, upper_boundL, max_exp_env. *)
+      (*       erewrite <- sizeOf_env_set_proj; eauto. *)
+      (*       eapply IHe; [ | | | | | | | | | eassumption ]. *)
+      (*       * eapply cc_approx_env_P_extend. *)
+      (*         eapply cc_approx_env_P_antimon; [ eassumption |]... *)
+      (*         eassumption. *)
+      (*       * now eauto. *)
+      (*       * eapply binding_in_map_antimon; [| eapply binding_in_map_set; eassumption ]. *)
+      (*         eapply occurs_free_Eproj_Included.  *)
+      (*       * intros f Hfin. eauto. *)
+      (*       * eapply injective_subdomain_antimon; eauto; sets. *)
+      (*       * eapply Disjoint_Included_r; *)
+      (*         [| eapply Disjoint_Included_l; [ apply image_monotonic | now apply Hd ]]. *)
+      (*         normalize_bound_var... now eauto with Ensembles_DB. *)
+      (*       * eapply Fun_inv_set_In_Scope_l. now eauto. *)
+      (*         eapply Fun_inv_set_In_Scope_r_not_Γ. now eauto. *)
+      (*         intros Heq; subst. now eauto. *)
+      (*         eapply Fun_inv_mon; [ | now eauto ]. *)
+      (*         eapply Disjoint_Included; [ | | now apply Hd ]. *)
+      (*         normalize_bound_var... sets. *)
+      (*       * eapply FV_inv_set_In_Scope_l. now constructor. *)
+      (*         eapply FV_inv_set_r. intros Hc. eapply Hnin. *)
+      (*         subst. now eauto. now eapply FV_inv_extend_Scope_GFuns. *)
+      (*       * eapply GFun_inv_set_not_In_GFuns_l. *)
+      (*         now intros Hc; inv Hc; eauto. *)
+      (*         eapply GFun_inv_set_not_In_GFuns_r. *)
+      (*         intros Hc. eapply Hd. constructor. *)
+      (*         rewrite image_Union. right. eapply image_monotonic; eauto... *)
+      (*         normalize_bound_var... sets. *)
+      (*         eapply GFun_inv_Scope_extend; sets. *)
+      (*         eapply Disjoint_Included; [| | now eapply Hd ]. *)
+      (*         normalize_bound_var... sets.  *)
+      (*         eapply GFun_inv_antimon; sets. }  *)
+      (* { intros c1 c2. unfold P, boundL, lower_boundL, upper_boundL. *)
+      (*   intros [Hle1 Hle2]; split; try omega. *)
+      (*   eapply le_trans; [| eapply plus_le_compat_r; eapply mult_le_compat_l; now apply max_exp_env_Eproj ]. *)
+      (*   simpl. omega. } *)
       admit. 
     - (* Case Efun -- the hardest one! *)
       inv Hcc.
@@ -2142,33 +1522,30 @@ Section Closure_conversion_correct.
       eapply cc_approx_val_monotonic; try eassumption. omega.
     - (* Case Eapp *)
       inv Hcc.
-      assert(Hadm : sizeOf_exp_ctx C <= 3 * length l + 3)
+      assert(Hadm : sizeOf_exp_ctx C <= 4 * length l + 4)
         by (eapply le_trans; [ now eapply project_vars_sizeOf_ctx_exp; eauto | simpl; omega ]).
       pose (P :=
               fun n c1 c2 : nat =>
-                c1 + n <= c2 + sizeOf_exp_ctx C <= 7 * c1 * max_exp_env k (Eapp v t l) rho1
-                                                 + 7 * sizeOf_exp (Eapp v t l) 
+                c1 + n <= c2 + sizeOf_exp_ctx C <= 8 * c1 * max_exp_env k (Eapp v t l) rho1
+                                                 + 8 * sizeOf_exp (Eapp v t l) 
                                                  + n).
       eapply cc_approx_exp_rel_mon with (P1 := P (sizeOf_exp_ctx C));
         [| intros n1 n2; unfold P, boundL, upper_boundL, lower_boundL; simpl; omega ].
       { intros v1 c1 Hleq Hstep. assert (Hstep' := Hstep); inv Hstep'.
         edestruct project_vars_ctx_to_rho as [rho2' Hto_rho]; eauto.
         simpl. rewrite H4, H5. reflexivity.
-        edestruct project_vars_correct as [Happ [Hfun' [Henv' Hvar]]]; eauto.
+        edestruct project_vars_correct as [Happ [Hfun' [Hgfun' [Henv' Hvar]]]]; eauto.
         edestruct Hvar as [v' [Hget' Happ']]; eauto.
         simpl. rewrite H4, H5. reflexivity.
         simpl in Hget'. destruct (M.get f' rho2') eqn:Hgetf'; try discriminate.
         destruct (get_list ys' rho2') eqn:Hget_list'; try discriminate. inv Hget'.
-        inv Happ'. rewrite cc_approx_val_eq in H6. destruct v0; try contradiction.
+        inv Happ'. rewrite cc_approx_val_eq in H6. destruct v0; try contradiction. 
         eapply ctx_to_rho_cc_approx_exp with (P' := P 0);
           [ now firstorder
           | now (intros n1 n2; simpl; unfold P; intros; omega) | | | | ]; try eassumption.
-        intros v1' c1' Hleq' Hstep'. inv Hstep'.
-        rewrite H4 in H8. inv H8. rewrite H5 in H15; inv H15.
+        intros v1' c1' Hleq' Hstep'. inv Hstep'. repeat subst_exp.
         destruct l1; try contradiction. destruct v0, l1; try contradiction.
-        destruct v2; try contradiction. 
-        rewrite H17 in H7. inv H7. 
-        rewrite H11 in H20. inv H20. eapply bstep_cost_deterministic in H21.
+        destruct v2; try contradiction. eapply bstep_cost_deterministic in H21.
         2:eapply H12. inv H21.
         assert (Hlen := List_util.Forall2_length _ _ _ H9).
         edestruct H6 with (vs2 := l0) (j := k - 1)
@@ -2181,26 +1558,27 @@ Section Closure_conversion_correct.
         - subst.
           assert (Heq: length ys' = length l).
           { symmetry. do 2 (erewrite get_list_length_eq; [| eassumption ]).
-            eapply Forall2_length. eassumption. }
+            eapply Forall2_length. eassumption. } 
           repeat eexists.
           + econstructor. eassumption. reflexivity.
-            econstructor. rewrite M.gso. eassumption.
-            intros Hc; subst. eapply project_vars_not_In_free_set; [ now eauto | now eauto | ].
-            constructor. now eapply H10. rewrite FromList_cons. now eauto.
+            econstructor. rewrite M.gso. eassumption. 
+            intros Hc; subst.  
+            eapply project_vars_not_In_free_set; [ eassumption | | ].
+            eassumption. eauto. constructor. now eapply H11. now left.
             reflexivity.
             eapply BStepc_app. rewrite M.gso. rewrite M.gss. reflexivity.
             now eauto.
             simpl. rewrite M.gss. rewrite get_list_set_neq. rewrite get_list_set_neq.
             rewrite Hget_list'. reflexivity. 
             intros Hin. eapply project_vars_not_In_free_set. eassumption. eassumption. 
-            constructor. eapply H10. rewrite FromList_cons. now eauto.
+            constructor. eapply H11. rewrite FromList_cons. now eauto.
             intros Hin. eapply project_vars_not_In_free_set. eassumption. eassumption.
             constructor. now eauto. rewrite FromList_cons. now eauto.
             eassumption. simpl in Hset. eauto. eassumption. 
           + simpl. unfold boundG, boundL, upper_boundL, lower_boundL in Hle1.
             omega.
           + unfold boundG, boundL, upper_boundL, lower_boundL in Hle2.
-            assert (Hles : sizeOf_exp e <= sizeOf_env k rho1).
+            assert (Hles : sizeOf_exp e0 <= sizeOf_env k rho1).
             { eapply le_trans; [| now eapply sizeOf_env_get; eauto ].
               destruct k; try omega. simpl. eapply le_trans. 
               eapply fun_in_fundefs_sizeOf_exp; eauto. now eapply find_def_correct; eauto.
@@ -2222,19 +1600,19 @@ Section Closure_conversion_correct.
           + eapply cc_approx_val_monotonic. eassumption. omega. }
     (* Case Eprim *)
     - inv Hcc.
-      assert(Hadm : sizeOf_exp_ctx C <= 3*length l) by (eapply project_vars_sizeOf_ctx_exp; eauto).
+      assert(Hadm : sizeOf_exp_ctx C <= 4 * length l) by (eapply project_vars_sizeOf_ctx_exp; eauto).
       pose (P :=
               fun n c1 c2 : nat =>
-                c1 + n <= c2 + sizeOf_exp_ctx C <= 7 * c1 * max_exp_env k e rho1
-                                                 + 7 * sizeOf_exp e + n).
+                c1 + n <= c2 + sizeOf_exp_ctx C <= 8 * c1 * max_exp_env k e rho1
+                                                 + 8 * sizeOf_exp e + n).
       eapply cc_approx_exp_rel_mon with (P1 := P (sizeOf_exp_ctx C)).
       { intros v1 c1 Hleq Hstep. assert (Hstep' := Hstep). inv Hstep'.
         edestruct project_vars_ctx_to_rho as [rho2' Hto_rho]; eauto.
-        edestruct project_vars_correct as [Happ [Hfun' [Henv' Hvar]]]; eauto.
+        edestruct project_vars_correct as [Happ [Hfun' [Hgfun' [Henv' Hvar]]]]; eauto.
         edestruct Hvar as [v' [Hget' Happ']]; eauto.
         eapply ctx_to_rho_cc_approx_exp with (P' := P 0); eauto.
         - now firstorder.
-        - now firstorder.
+        - clear; now firstorder.
         - eapply cc_approx_exp_prim_compat with (S0 := boundL k e rho1).
           + unfold boundL, upper_boundL, lower_boundL, P. intros c1 c2 n Hle.
             rewrite <- !plus_n_O. intros [Hle1 Hle2]; split; try omega.
@@ -2242,13 +1620,13 @@ Section Closure_conversion_correct.
             eapply plus_le_compat; eauto. eapply plus_le_mult; eauto.
             now apply max_exp_env_grt_1. eapply le_trans. eassumption.
             omega.
-          + eapply Forall2_cc_approx_var_env; eauto.
+          + eapply Forall2_cc_approx_var_env; eauto. 
           + intros vs1 vs2 l1 f Hgetl Hgetf Happf Hall.
             unfold boundL, upper_boundL, lower_boundL, max_exp_env.
             assert (HadmX : sizeOf_env k rho1 = sizeOf_env k (M.set  v vs1 rho1)).
             { erewrite sizeOf_env_set, primAxiom; eauto. }
             erewrite HadmX; eauto.
-            eapply IHe; [ | | | | eassumption | | | | eassumption ].
+            eapply IHe with (c := c'); [ | | | | | | | | | eassumption ].
             * eapply cc_approx_env_P_extend with (v2 := vs2).
               eapply cc_approx_env_P_antimon; [ eassumption |]...
               eassumption.
@@ -2256,16 +1634,26 @@ Section Closure_conversion_correct.
             * eapply binding_in_map_antimon; [| eapply binding_in_map_set; eassumption ].
               eapply occurs_free_Eprim_Included. 
             * intros f1 Hfin. eauto.
+            * eapply injective_subdomain_antimon. eassumption. sets. 
             * eapply Disjoint_Included_r;
               [| eapply Disjoint_Included_l; [ apply image_monotonic | now apply Hd ]].
               normalize_bound_var... now eauto with Ensembles_DB.
             * eapply Fun_inv_set_In_Scope_l. now eauto.
               eapply Fun_inv_set_In_Scope_r_not_Γ. now eauto.
               intros Heq; subst. now eauto.
-              eapply Fun_inv_mon; [ | now eauto ]...
+              eapply Fun_inv_mon; [ | now eauto ].
+              eapply Disjoint_Included; [| | eapply Hd ]; sets.
             * eapply FV_inv_set_In_Scope_l. now constructor.
               eapply FV_inv_set_r. intros Hc. eapply Hnin.
-              subst. now eauto. now eapply FV_inv_extend_Scope. }
+              subst. now eauto. now eapply FV_inv_extend_Scope_GFuns.
+            * eapply GFun_inv_set_not_In_GFuns_l. intros Hc. inv Hc. eapply H0. reflexivity.
+              eapply GFun_inv_set_not_In_GFuns_r.
+              intros Hc. eapply Hd. constructor. rewrite image_Union.
+              right. eapply image_monotonic; [| eassumption ]; sets. sets.
+              eapply GFun_inv_Scope_extend; sets.
+              eapply Disjoint_Included; [| | now eapply Hd ].
+              normalize_bound_var... sets. 
+              eapply GFun_inv_antimon; sets. } 
       { intros c1 c2. unfold P, boundL, lower_boundL, upper_boundL.
         intros [Hle1 Hle2]; split; try omega.
         eapply le_trans;
@@ -2273,19 +1661,21 @@ Section Closure_conversion_correct.
         simpl. omega. }
    (* Case Ehalt *)
     - inv Hcc.
-      assert(Hadm : sizeOf_exp_ctx C <= 3) by (eapply project_var_sizeOf_ctx_exp; eauto).
+      assert(Hadm : sizeOf_exp_ctx C <= 4) by (eapply project_var_sizeOf_ctx_exp; eauto).
       pose (P :=
               fun n c1 c2 : nat =>
-                c1 + n <= c2 + sizeOf_exp_ctx C <= 7 * c1 * max_exp_env k (Ehalt v) rho1
-                                                 + 7 + n).
+                c1 + n <= c2 + sizeOf_exp_ctx C <= 8 * c1 * max_exp_env k (Ehalt v) rho1
+                                                 + 8 + n).
       eapply cc_approx_exp_rel_mon with (P1 := P (sizeOf_exp_ctx C)).
       { intros v1 c1 Hleq Hstep. assert (Hstep' := Hstep). inv Hstep'.
         edestruct project_var_ctx_to_rho as [rho2' Hto_rho]; eauto.
-        edestruct project_var_correct as [Hnin' [Happ [Hfun' [Henv' Hvar]]]]; eauto.
+        eapply Disjoint_Included_r; [| eassumption ]. rewrite image_Union.
+        eauto 10 with Ensembles_DB.
+        edestruct project_var_correct as [Hnin' [Happ [Hfun' [Hgfun' [Henv' Hvar]]]]]; eauto.
         edestruct Hvar as [v' [Hget' Happ']]; eauto.
         eapply ctx_to_rho_cc_approx_exp with (P' := P 0); eauto.
         - now firstorder.
-        - now firstorder.
+        - clear. now firstorder.
         - eapply cc_approx_exp_halt_compat.
           unfold P. omega.
           eassumption. }
